proof/old_system/uni/decl_worklist/def.v
@@ -73,6 +73,54 @@ Inductive d_wl_del_red : dworklist -> Prop :=
       d_wl_del_red (dworklist_conswork Ω (work_applyd cd A B))
   .
 
+Fixpoint iuv_size (A : typ) : nat :=
+  match A with
+  | typ_var_b _ => 1
+  | typ_arrow A1 A2 => iuv_size A1 + iuv_size A2
+  | typ_all A => iuv_size A
+  | typ_union A1 A2 => 1 + iuv_size A1 + iuv_size A2
+  | typ_intersection A1 A2 => 1 + iuv_size A1 + iuv_size A2
+  | _ => 0
+  end.
+
+Fixpoint lookup_bind (Γ : aenv) (X : atom) : option typ :=
+  match Γ with
+  | nil => None
+  | (Y, abind_var_typ A) :: Γ' => if X == Y then Some A else lookup_bind Γ' X
+  | (_, _) :: Γ' => lookup_bind Γ' X
+  end.
+
+Fixpoint exp_split_size (Γ : aenv) (e : exp) : nat :=
+  match e with
+  | exp_unit => 0
+  | exp_var_b _ => 0
+  | exp_var_f X => match lookup_bind Γ X with
+                  | Some A => iuv_size A
+                  | None => 0
+                  end
+  | exp_abs e1 => exp_split_size Γ e1
+  | exp_app e1 e2 => 1 + 2 * exp_split_size Γ e1 + exp_split_size Γ e2
+  | exp_tabs (body_anno e1 A) => (1 + exp_split_size Γ e1) * (2 + iuv_size A)
+  | exp_tapp e1 A => (1 + exp_split_size Γ e1) * (2 + iuv_size A)
+  | exp_anno e1 A => (1 + exp_split_size Γ e1) * (2 + iuv_size A)
+  end.
+
+
+Definition dbind_to_abind (d : dbind) : abind :=
+  match d with
+  | dbind_typ A => abind_var_typ A
+  | dbind_stvar_empty => abind_stvar_empty
+  | dbind_tvar_empty => abind_tvar_empty
+  end.
+
+Fixpoint dwl_to_aenv (dW : dworklist) : aenv :=
+  match dW with 
+  | dworklist_empty => nil
+  | dworklist_conswork dW' _ => dwl_to_aenv dW'
+  | dworklist_constvar dW' X b => X ~ (dbind_to_abind b) ++ dwl_to_aenv dW'
+  | dworklist_consvar dW' x b => x ~ (dbind_to_abind b) ++ dwl_to_aenv dW'
+  end.
+
 (* defns Jdworklist_reduction *)
 Inductive d_wl_red : dworklist -> Prop :=    (* defn d_wl_red *)
  | d_wl_red__empty : d_wl_red dworklist_empty
@@ -172,8 +220,8 @@ Inductive d_wl_red : dworklist -> Prop :=    (* defn d_wl_red *)
      (forall x, x `notin` L ->
         d_wl_red (dworklist_conswork (dworklist_consvar (dworklist_conswork Ω (work_applys cs (typ_arrow T1 T2))) x (dbind_typ T1)) (work_check (open_exp_wrt_exp e (exp_var_f x)) T2))) ->
      d_wl_red (dworklist_conswork Ω (work_infer (exp_abs e) cs))
- | d_wl_red__inf_app : forall (Ω:dworklist) (e1 e2:exp) (cs:conts),
-     d_wl_red (dworklist_conswork Ω (work_infer e1 (conts_infabs (contd_infapp e2 cs)))) ->
+ | d_wl_red__inf_app : forall (Ω:dworklist) (e1 e2:exp) (cs:conts) (n:nat),
+     d_wl_red (dworklist_conswork Ω (work_infer e1 (conts_infabs (contd_infapp (exp_split_size (dwl_to_aenv Ω) e1) e2 cs)))) ->
      d_wl_red (dworklist_conswork Ω (work_infer  ( (exp_app e1 e2) )  cs))
  | d_wl_red__inf_tapp : forall (Ω:dworklist) (e:exp) (B:typ) (cs:conts),
      d_wl_red (dworklist_conswork Ω (work_infer e (conts_inftapp B cs))) ->
